@prefix : <http://courseweb.lis.illinois.edu/lis/2015sp/lis590odl/gslis/> .
@prefix dc: <http://purl.org/dc/elements/1.1/> .
@prefix tl: <http://purl.org/NET/c4dm/timeline.owl#> .
@prefix dbp: <http://dbpedia.org/resource/> .
@prefix geo: <http://www.w3.org/2003/01/geo/wgs84_pos#> .
@prefix org: <http://www.w3.org/ns/org#> .
@prefix owl: <http://www.w3.org/2002/07/owl#> .
@prefix rdf: <http://www.w3.org/1999/02/22-rdf-syntax-ns#> .
@prefix xml: <http://www.w3.org/XML/1998/namespace> .
@prefix xsd: <http://www.w3.org/2001/XMLSchema#> .
@prefix xsp: <http://www.owl-ontologies.com/2005/08/07/xsp.owl#> .
@prefix foaf: <http://xmlns.com/foaf/0.1/> .
@prefix prov: <http://www.w3.org/ns/prov#> .
@prefix rdfs: <http://www.w3.org/2000/01/rdf-schema#> .
@prefix skos: <http://www.w3.org/2004/02/skos/core#> .
@prefix swrl: <http://www.w3.org/2003/11/swrl#> .
@prefix wped: <http://en.wikipedia.org/wiki/> .
@prefix dolce: <http://ontology.ip.rm.cnr.it/ontologies/DOLCE-Lite#> .
@prefix event: <http://purl.org/NET/c4dm/event.owl#> .
@prefix gslis: <http://courseweb.lis.illinois.edu/lis/2015sp/lis590odl/RDF/gslis.ttl> .
@prefix swrlb: <http://www.w3.org/2003/11/swrlb#> .
@prefix dcterms: <http://purl.org/dc/terms/> .
@prefix protege: <http://protege.stanford.edu/plugins/owl/protege#> .
@base <http://people.lis.illinois.edu/~dforero2/LIS590ODL/dforero2.ttl> .

<http://people.lis.illinois.edu/~dforero2/LIS590ODL/dforero2.ttl> rdf:type owl:Ontology ;
                                                                  
                                                                  dc:title "GSLIS Forero Ontology" ;
                                                                  
                                                                  owl:imports <http://courseweb.lis.illinois.edu/lis/2015sp/lis590odl/RDF/gslis.ttl> ,
                                                                              <http://purl.org/NET/c4dm/event.owl> ,
                                                                              <http://www.w3.org/2004/02/skos/core> ,
                                                                              org: ,
                                                                              foaf: .


#################################################################
#
#    Object Properties
#
#################################################################


###  http://courseweb.lis.illinois.edu/lis/2015sp/lis590odl/gslis/hasPrerequisite

:hasPrerequisite rdf:type owl:ObjectProperty ;
                 
                 rdfs:comment "has an object course that must be completed before enrolling in subject course."@en ;
                 
                 rdfs:domain :Course ;
                 
                 rdfs:range :Course .



###  http://courseweb.lis.illinois.edu/lis/2015sp/lis590odl/gslis/hasRelatedCourse

:hasRelatedCourse rdf:type owl:ObjectProperty ;
                  
                  rdfs:comment "has a relation between programs and related courses"@en ;
                  
                  rdfs:domain :Program ;
                  
                  rdfs:range :RelatedCourse .





#################################################################
#
#    Data properties
#
#################################################################


###  http://courseweb.lis.illinois.edu/lis/2015sp/lis590odl/gslis/hasCourseID

:hasCourseID rdf:type owl:DatatypeProperty ;
             
             rdfs:comment "has an unique identifier of the course made up of the department abbreviation a three digit number and an option abbreviation for a particular variation of the course."@en ;
             
             rdfs:domain :Course ;
             
             rdfs:range xsd:string .



###  http://courseweb.lis.illinois.edu/lis/2015sp/lis590odl/gslis/hasCourseName

:hasCourseName rdf:type owl:DatatypeProperty ;
               
               rdfs:comment "has a full name of course without abbreviation."@en ;
               
               rdfs:domain :Course ;
               
               rdfs:range xsd:string .



###  http://courseweb.lis.illinois.edu/lis/2015sp/lis590odl/gslis/hasCredit

:hasCredit rdf:type owl:DatatypeProperty ;
           
           rdfs:comment "has an integer value of credits for course"@en ;
           
           rdfs:domain :Course ;
           
           rdfs:range xsd:nonNegativeInteger .



###  http://courseweb.lis.illinois.edu/lis/2015sp/lis590odl/gslis/hasCreditType

:hasCreditType rdf:type owl:DatatypeProperty ;
               
               rdfs:comment "has a kind of credit either UG (Undergraduate) or GR (Graduate)."@en ;
               
               rdfs:domain :Course ;
               
               rdfs:subPropertyOf :hasCredit ;
               
               rdfs:range xsd:string .



###  http://courseweb.lis.illinois.edu/lis/2015sp/lis590odl/gslis/hasDescription

:hasDescription rdf:type owl:DatatypeProperty ;
                
                rdfs:comment "has description for the curriculum and themes of the course content."@en ;
                
                rdfs:domain :Course ;
                
                rdfs:range xsd:string .



###  http://courseweb.lis.illinois.edu/lis/2015sp/lis590odl/gslis/hasRelatedCourseQuantity

:hasRelatedCourseQuantity rdf:type owl:DatatypeProperty ;
                          
                          rdfs:comment "Integer value of number of courses required for a particular related set of courses in a program."@en ;
                          
                          rdfs:domain :hasRelatedCourse ;
                          
                          rdfs:range xsd:decimal .





#################################################################
#
#    Classes
#
#################################################################


###  http://courseweb.lis.illinois.edu/lis/2015sp/lis590odl/gslis/Course

:Course rdf:type owl:Class ;
        
        rdfs:subClassOf :Activity ;
        
        rdfs:comment "This class consists of specific program that are usually credit bearing and have a defined curriculum."@en .



###  http://courseweb.lis.illinois.edu/lis/2015sp/lis590odl/gslis/OtherProgram

:OtherProgram rdf:type owl:Class ;
              
              rdfs:subClassOf :Program_of_Study ;
              
              rdfs:comment "Programs that are not degree granting."@en .



###  http://courseweb.lis.illinois.edu/lis/2015sp/lis590odl/gslis/RelatedCourse

:RelatedCourse rdf:type owl:Class ;
               
               rdfs:subClassOf :Course ;
               
               rdfs:comment "Grouping of equivalent courses for a particular Program"@en .



###  http://courseweb.lis.illinois.edu/lis/2015sp/lis590odl/gslis/hasRelatedCourse

:hasRelatedCourse rdf:type owl:Class ;
                  
                  rdfs:comment "has a relation between programs and related courses"@en .



###  http://www.w3.org/2002/07/owl#subProperty

owl:subProperty rdf:type owl:Class .





#################################################################
#
#    Individuals
#
#################################################################


###  http://courseweb.lis.illinois.edu/lis/2015sp/lis590odl/gslis/hasRelatedCourseQuantity

:hasRelatedCourseQuantity rdf:type owl:NamedIndividual ,
                                   owl:subProperty ;
                          
                          rdfs:comment "Integer value of number of courses required for a particular related set of courses in a program."@en .




###  Generated by the OWL API (version 3.5.0) http://owlapi.sourceforge.net

