@prefix course: <https://github.com/f0rer0/course/blob/master/course.ttl> .
@prefix dc: <http://purl.org/dc/elements/1.1/> .
@prefix foaf: <http://xmlns.com/foaf/0.1/> .
@prefix gslis: <http://courseweb.lis.illinois.edu/lis/2015sp/lis590odl/gslis/> .
@prefix owl: <http://www.w3.org/2002/07/owl#> .
@prefix rdfs: <http://www.w3.org/2000/01/rdf-schema#> .
@prefix rdf: <http://www.w3.org/1999/02/22-rdf-syntax-ns#> .
@prefix org: <http://www.w3.org/ns/org#> .
@prefix xsd: <http://www.w3.org/2001/XMLSchema#> .

@base <https://github.com/f0rer0/course/blob/master/course.ttl> .

<https://github.com/f0rer0/course/blob/master/course.ttl> rdf:type owl:Ontology ;
                                                                  
                                                                  dc:title "GSLIS Course Ontology" ;
                                                                  
                                                                  owl:imports <http://courseweb.lis.illinois.edu/lis/2015sp/lis590odl/RDF/gslis.ttl> ,
                                                                              <http://purl.org/NET/c4dm/event.owl> ,
                                                                              <http://www.w3.org/2004/02/skos/core> ,
                                                                              org: ,
                                                                              foaf: .


#################################################################
#
#    Object Properties
#
#################################################################


###  http://courseweb.lis.illinois.edu/lis/2015sp/lis590odl/gslis/hasPrerequisite

course:hasPrerequisite rdf:type owl:ObjectProperty ;
                 
                 rdfs:comment "has an object course that must be completed before enrolling in subject course."@en ;
                 
                 rdfs:domain course:Course ;
                 
                 rdfs:range course:Course .



###  http://courseweb.lis.illinois.edu/lis/2015sp/lis590odl/gslis/hasRelatedCourse

course:hasRelatedCourse rdf:type owl:ObjectProperty ;
                  
                  rdfs:comment "has a relation between programs and related courses"@en ;
                  
                  rdfs:domain gslis:Program ;
                  
                  rdfs:range course:RelatedCourse .





#################################################################
#
#    Data properties
#
#################################################################


###  http://courseweb.lis.illinois.edu/lis/2015sp/lis590odl/gslis/hasCourseID

course:hasCourseID rdf:type owl:DatatypeProperty ;
             
             rdfs:comment "has an unique identifier of the course made up of the department abbreviation a three digit number and an option abbreviation for a particular variation of the course."@en ;
             
             rdfs:domain course:Course ;
             
             rdfs:range xsd:string .



###  http://courseweb.lis.illinois.edu/lis/2015sp/lis590odl/gslis/hasCourseName

course:hasCourseName rdf:type owl:DatatypeProperty ;
               
               rdfs:comment "has a full name of course without abbreviation."@en ;
               
               rdfs:domain course:Course ;
               
               rdfs:range xsd:string .



###  http://courseweb.lis.illinois.edu/lis/2015sp/lis590odl/gslis/hasCredit

course:hasCredit rdf:type owl:DatatypeProperty ;
           
           rdfs:comment "has an integer value of credits for course"@en ;
           
           rdfs:domain course:Course ;
           
           rdfs:range xsd:nonNegativeInteger .



###  http://courseweb.lis.illinois.edu/lis/2015sp/lis590odl/gslis/hasCreditType

course:hasCreditType rdf:type owl:DatatypeProperty ;
               
               rdfs:comment "has a kind of credit either UG (Undergraduate) or GR (Graduate)."@en ;
               
               rdfs:domain course:Course ;
               
               rdfs:subPropertyOf course:hasCredit ;
               
               rdfs:range xsd:string .



###  http://courseweb.lis.illinois.edu/lis/2015sp/lis590odl/gslis/hasDescription

course:hasDescription rdf:type owl:DatatypeProperty ;
                
                rdfs:comment "has description for the curriculum and themes of the course content."@en ;
                
                rdfs:domain course:Course ;
                
                rdfs:range xsd:string .



###  http://courseweb.lis.illinois.edu/lis/2015sp/lis590odl/gslis/hasRelatedCourseQuantity

course:hasRelatedCourseQuantity rdf:type owl:DatatypeProperty ;
                          
                          rdfs:comment "Integer value of number of courses required for a particular related set of courses in a program."@en ;
                          
                          rdfs:domain course:hasRelatedCourse ;
                          
                          rdfs:range xsd:decimal .





#################################################################
#
#    Classes
#
#################################################################


###  http://courseweb.lis.illinois.edu/lis/2015sp/lis590odl/gslis/Course

course:Course rdf:type owl:Class ;
        
        rdfs:subClassOf gslis:Activity ;
        
        rdfs:comment "This class consists of specific program that are usually credit bearing and have a defined curriculum."@en .



###  http://courseweb.lis.illinois.edu/lis/2015sp/lis590odl/gslis/OtherProgram

course:OtherProgram rdf:type owl:Class ;
              
              rdfs:subClassOf gslis:Program_of_Study ;
              
              rdfs:comment "Programs that are not degree granting."@en .



###  http://courseweb.lis.illinois.edu/lis/2015sp/lis590odl/gslis/RelatedCourse

course:RelatedCourse rdf:type owl:Class ;
               
               rdfs:subClassOf course:Course ;
               
               rdfs:comment "Grouping of equivalent courses for a particular Program"@en .



###  http://courseweb.lis.illinois.edu/lis/2015sp/lis590odl/gslis/hasRelatedCourse

course:hasRelatedCourse rdf:type owl:Class ;
                  
                  rdfs:comment "has a relation between programs and related courses"@en .



###  http://www.w3.org/2002/07/owl#subProperty

owl:subProperty rdf:type owl:Class .





#################################################################
#
#    Individuals
#
#################################################################


###  http://courseweb.lis.illinois.edu/lis/2015sp/lis590odl/gslis/hasRelatedCourseQuantity

course:hasRelatedCourseQuantity rdf:type owl:NamedIndividual ,
                                   owl:subProperty ;
                          
                          rdfs:comment "Integer value of number of courses required for a particular related set of courses in a program."@en .




###  Generated by the OWL API (version 3.5.0) http://owlapi.sourceforge.net

